format-version: 1.2
data-version: https://www.inf.ufrgs.br/bdi/ontologies/geores/releases/2024-10-14/geores.owl
idspace: dce http://purl.org/dc/elements/1.1/ 
idspace: dcterms http://purl.org/dc/terms/ 
idspace: ontologies https://www.inf.ufrgs.br/bdi/ontologies/ 
idspace: skos http://www.w3.org/2004/02/skos/core# 
remark: Cited references:\n\n1. Abel, M., Perrin, M., Carbonera, J.L.: Ontological analysis for information integration in geomodeling. Earth Science Informatics 8, 21–36 (2015)\n2. Carbonera, J.L., Abel, M., Scherer, C.M.S.: Visual interpretation of events in petroleum exploration: An approach supported by well-founded ontologies. Expert Systems With Applications 42, 2749–2763 (2015)\n3. Cullis, S., Colombera, L., Patacci, M., McCaffrey, W.D.: Hierarchical classifications of the sedimentary architecture of deep-marine depositional systems. Earth-Science Reviews 179, 38–71 (2018)\n4. De Ros, L.F., Goldberg, K.: Reservoir petrofacies: A tool for quality characterization and prediction. In: AAPG Annual Conference and Exhibition. Long Beach (2007)\n5. Garcia, L.F., Carbonera, J.L., Rodrigues, F.H., Antunes, C.R., Abel, M.: What rocks are made of: Towards an ontological pattern for material constitution in the geological domain. In: Laender, A.H.F., Pernici, B., Lim, E.P., Oliveira, J.P.M. (eds.) ER: 38th International Conference on Conceptual Modeling. pp. 275–286. Springer, Cham (2019)\n6. Guarino, N., Welty, C.A.: An overview of ontoclean. In: Staab, S., Studer, R. (eds.) Handbook on Ontologies, pp. 151–171. Springer, Berlin, Heidelberg (2004)\n7. McHargue, T., Pyrcz, M.J., Sullivan, M.D., Clark, J.D., Fildani, A., Romans, B.W., Covault, J.A., Levy, M., Posamentier, H.W., Drinkwater, N.J.: Architecture of turbidite channel systems on the continental slope: Patterns and predictions. Marine and Petroleum Geology 28, 728–743 (2011)\n8. Middleton, G.V.: Johannes walther’s law of the correlation of facies. Bulletin of the Geological Society of America 84, 979–988 (1973)\n9. Nichols, G.: Sedimentology and Stratigraphy. Wiley-Blackwell, Chichester, 2nd edn. (2009)\n10. Rovetto, R.: The shape of shapes: An ontological exploration. In: Hastings, J., Kutz, O., Bhatt, M., Borgo, S. (eds.) Proceedings of the First Interdisciplinary Workshop on SHAPES. Karlsruhe (2011), http://ceur-ws.org/Vol-812/\n11. Walker, R.G., James, N.P.: Facies Models: Response to Sea Level Change. Geological Association of Canada, St. John’s (1992)
remark: We acknowledge the Brazilian funding agencies CNPq and CAPES for financing this work and the Research Centre of Petrobras (CENPES) for collaborating on this project.
ontology: https://www.inf.ufrgs.br/bdi/ontologies/geores.owl
property_value: dce:contributor "Alcides Lopes" xsd:string
property_value: dce:contributor "Fabrício Henrique Rodrigues" xsd:string
property_value: dce:contributor "Fernando Cicconeto" xsd:string
property_value: dce:contributor "Joel Luis Carbonera" xsd:string
property_value: dce:contributor "Luan Fonseca Garcia" xsd:string
property_value: dce:contributor "Lucas Valadares Vieira" xsd:string
property_value: dce:contributor "Mara Abel" xsd:string
property_value: dce:contributor "Renata dos Santos Alvarenga" xsd:string
property_value: dce:contributor "Tiago Agne de Oliveira" xsd:string
property_value: dce:contributor "Yuanwei Qu" xsd:string
property_value: dcterms:description "GeoReservoir is an ontology to support the description of the geometry and the lithology of deep-marine deposits. The GeoReservoir ontology provides formal and clear definitions of deep-marine depositional system entities, creating an unambiguous terminology for geometrical and lithological properties of the deposits in the scale of outcrop and seismic sections. These definitions are independent of tasks, geological interpretations, and process inferences. We created this language to make it possible to formally and uniformly describe any deep-marine occurrence in the world with an adequate level of detail for sedimentological studies and computer processing." xsd:string
property_value: dcterms:license "https://creativecommons.org/licenses/by-nc/4.0/" xsd:string
property_value: dcterms:title "GeoReservoir Ontology" xsd:string
property_value: owl:versionInfo "2024-10-14" xsd:string

[Term]
id: BFO:0000001
name: entity
property_value: dce:identifier "001-BFO" xsd:string
property_value: skos:definition "(Elucidation) An entity is anything that exists or has existed or will exist" xsd:string
property_value: skos:example "Julius Caesar; the Second World War; your body mass index; Verdi's Requiem" xsd:string

[Term]
id: BFO:0000002
name: continuant
is_a: BFO:0000001 ! entity
disjoint_from: BFO:0000003 ! occurrent
relationship: BFO:0000176 BFO:0000002 {all_only="true"} ! continuant part of continuant
property_value: dce:identifier "008-BFO" xsd:string
property_value: skos:definition "(Elucidation) A continuant is an entity that persists, endures, or continues to exist through time while maintaining its identity" xsd:string
property_value: skos:example "A human being; a tennis ball; a cave; a region of space; someone's temperature" xsd:string

[Term]
id: BFO:0000003
name: occurrent
is_a: BFO:0000001 ! entity
property_value: dce:identifier "077-BFO" xsd:string
property_value: skos:definition "(Elucidation) An occurrent is an entity that unfolds itself in time or it is the start or end of such an entity or it is a temporal or spatiotemporal region" xsd:string
property_value: skos:example "As for process, history, process boundary, spatiotemporal region, zero-dimensional temporal region, one-dimensional temporal region, temporal interval, temporal instant." xsd:string

[Term]
id: BFO:0000004
name: independent continuant
is_a: BFO:0000002 ! continuant
disjoint_from: BFO:0000020 ! specifically dependent continuant
relationship: BFO:0000176 BFO:0000004 {all_only="true"} ! continuant part of independent continuant
property_value: dce:identifier "017-BFO" xsd:string
property_value: skos:definition "b is an independent continuant =Def b is a continuant & there is no c such that b specifically depends on c or b generically depends on c" xsd:string
property_value: skos:example "An atom; a molecule; an organism; a heart; a chair; the bottom right portion of a human torso; a leg; the interior of your mouth; a spatial region; an orchestra" xsd:string

[Term]
id: BFO:0000006
name: spatial region
is_a: BFO:0000141 ! immaterial entity
disjoint_from: BFO:0000029 ! site
relationship: BFO:0000176 BFO:0000006 {all_only="true"} ! continuant part of spatial region
property_value: dce:identifier "035-BFO" xsd:string
property_value: skos:definition "(Elucidation) A spatial region is a continuant entity that is a continuant part of the spatial projection of a portion of spacetime at a given time" xsd:string
property_value: skos:example "As for zero-dimensional spatial region, one-dimensional spatial region, two-dimensional spatial region, three-dimensional spatial region" xsd:string

[Term]
id: BFO:0000008
name: temporal region
is_a: BFO:0000003 ! occurrent
disjoint_from: BFO:0000011 ! spatiotemporal region
property_value: dce:identifier "100-BFO" xsd:string
property_value: skos:definition "(Elucidation) A temporal region is an occurrent over which processes can unfold" xsd:string
property_value: skos:example "As for zero-dimensional temporal region and one-dimensional temporal region" xsd:string

[Term]
id: BFO:0000011
name: spatiotemporal region
is_a: BFO:0000003 ! occurrent
property_value: dce:identifier "095-BFO" xsd:string
property_value: skos:definition "(Elucidation) A spatiotemporal region is an occurrent that is an occurrent part of spacetime" xsd:string
property_value: skos:example "The spatiotemporal region occupied by the development of a cancer tumour; the spatiotemporal region occupied by an orbiting satellite" xsd:string
property_value: skos:scopeNote "'Spacetime' here refers to the maximal instance of the universal spatiotemporal region." xsd:string

[Term]
id: BFO:0000015
name: process
is_a: BFO:0000003 ! occurrent
property_value: dce:identifier "083-BFO" xsd:string
property_value: skos:altLabel "event" xsd:string
property_value: skos:definition "(Elucidation) p is a process means p is an occurrent that has some temporal proper part and for some time t, p has some material entity as participant" xsd:string
property_value: skos:example "An act of selling; the life of an organism; a process of sleeping; a process of cell-division; a beating of the heart; a process of meiosis; the taxiing of an aircraft; the programming of a computer" xsd:string

[Term]
id: BFO:0000019
name: quality
is_a: BFO:0000020 ! specifically dependent continuant
property_value: dce:identifier "055-BFO" xsd:string
property_value: skos:definition "(Elucidation) A quality is a specifically dependent continuant that, in contrast to roles and dispositions, does not require any further process in order to be realized" xsd:string
property_value: skos:example "The colour of a tomato; the ambient temperature of this portion of air; the length of the circumference of your waist; the shape of your nose; the shape of your nostril; the mass of this piece of gold" xsd:string

[Term]
id: BFO:0000020
name: specifically dependent continuant
is_a: BFO:0000002 ! continuant
property_value: dce:identifier "050-BFO" xsd:string
property_value: skos:definition "b is a specifically dependent continuant =Def b is a continuant & there is some independent continuant c which is not a spatial region & which is such that b specifically depends on c" xsd:string
property_value: skos:example "(with multiple bearers) John's love for Mary; the ownership relation between John and this statue; the relation of authority between John and his subordinates" xsd:string
property_value: skos:example "(with one bearer) The mass of this tomato; the pink colour of a medium rare piece of grilled filet mignon at its centre; the smell of this portion of mozzarella; the disposition of this fish to decay; the role of being a doctor; the function of this heart to pump blood; the shape of this hole" xsd:string

[Term]
id: BFO:0000027
name: object aggregate
is_a: BFO:0000040 ! material entity
property_value: dce:identifier "025-BFO" xsd:string
property_value: skos:definition "(Elucidation) An object aggregate is a material entity consisting exactly of a plurality (≥1) of objects as member parts which together form a unit" xsd:string
property_value: skos:example "The aggregate of the musicians in a symphony orchestra and their instruments; the aggregate of bearings in a constant velocity axle joint; the nitrogen atoms in the atmosphere; a collection of cells in a blood biobank" xsd:string
property_value: skos:scopeNote "'Exactly' means that there are no parts of the object aggregate other than its member parts." xsd:string
property_value: skos:scopeNote "The unit can, at certain times, consist of exactly one object, for example, when a wolf litter loses all but one of its pups, but it must at some time have a plurality of member parts." xsd:string

[Term]
id: BFO:0000029
name: site
is_a: BFO:0000141 ! immaterial entity
property_value: dce:identifier "034-BFO" xsd:string
property_value: skos:definition "(Elucidation) A site is a three-dimensional immaterial entity whose boundaries either (partially or wholly) coincide with the boundaries of one or more material entities or have locations determined in relation to some material entity" xsd:string
property_value: skos:example "A hole in a portion of cheese; a rabbit hole; the Grand Canyon; the Piazza San Marco; the kangaroo-joey-containing hole of a kangaroo pouch; your left nostril (a fiat part - the opening - of your left nasal cavity); the lumen of your gut; the hold of a ship; the interior of the trunk of your car; hole in an engineered floor joist" xsd:string

[Term]
id: BFO:0000030
name: object
is_a: BFO:0000040 ! material entity
property_value: dce:identifier "024-BFO" xsd:string
property_value: skos:definition "(Elucidation) An object is a material entity which manifests causal unity & is of a type instances of which are maximal relative to the sort of causal unity manifested" xsd:string
property_value: skos:example "An organism; a fish tank; a planet; a laptop; a valve; a block of marble; an ice cube" xsd:string
property_value: skos:scopeNote "A description of three primary sorts of causal unity is provided in Basic Formal Ontology 2.0. Specification and User Guide" xsd:string

[Term]
id: BFO:0000031
name: generically dependent continuant
is_a: BFO:0000002 ! continuant
property_value: dce:identifier "074-BFO" xsd:string
property_value: skos:altLabel "g-dependent continuant" xsd:string
property_value: skos:definition "(Elucidation) A generically dependent continuant is an entity that exists in virtue of the fact that there is at least one of what may be multiple copies which is the content or the pattern that multiple copies would share" xsd:string
property_value: skos:example "The pdf file on your laptop; the pdf file that is a copy thereof on my laptop; the sequence of this protein molecule; the sequence that is a copy thereof in that protein molecule; the content that is shared by a string of dots and dashes written on a page and the transmitted Morse code signal; the content of a sentence; an engineering blueprint" xsd:string

[Term]
id: BFO:0000035
name: process boundary
is_a: BFO:0000003 ! occurrent
property_value: dce:identifier "084-BFO" xsd:string
property_value: skos:definition "p is a process boundary =Def p is a temporal part of a process & p has no proper temporal parts" xsd:string
property_value: skos:example "The boundary between the 2nd and 3rd year of your life" xsd:string

[Term]
id: BFO:0000038
name: one-dimensional temporal region
is_a: BFO:0000008 ! temporal region
property_value: dce:identifier "103-BFO" xsd:string
property_value: skos:definition "(Elucidation) A one-dimensional temporal region is a temporal region that is a whole that has a temporal interval and zero or more temporal intervals and temporal instants as parts" xsd:string
property_value: skos:example "The temporal region during which a process occurs" xsd:string

[Term]
id: BFO:0000040
name: material entity
is_a: BFO:0000004 ! independent continuant
disjoint_from: BFO:0000141 ! immaterial entity
relationship: BFO:0000176 BFO:0000040 {all_only="true"} ! continuant part of material entity
property_value: dce:identifier "019-BFO" xsd:string
property_value: skos:definition "(Elucidation) A material entity is an independent continuant has some portion of matter as continuant part" xsd:string
property_value: skos:example "A human being; the undetached arm of a human being; an aggregate of human beings" xsd:string

[Term]
id: BFO:0000140
name: continuant fiat boundary
is_a: BFO:0000141 ! immaterial entity
relationship: BFO:0000178 BFO:0000140 {all_only="true"} ! has continuant part continuant fiat boundary
property_value: dce:identifier "029-BFO" xsd:string
property_value: skos:definition "(Elucidation) A continuant fiat boundary b is an immaterial entity that is of zero, one or two dimensions & such that there is no time t when b has a spatial region as continuant part & whose location is determined in relation to some material entity" xsd:string
property_value: skos:example "As for fiat point, fiat line, fiat surface" xsd:string

[Term]
id: BFO:0000141
name: immaterial entity
is_a: BFO:0000004 ! independent continuant
property_value: dce:identifier "028-BFO" xsd:string
property_value: skos:definition "b is an immaterial entity =Def b is an independent continuant which is such that there is no time t when it has a material entity as continuant part" xsd:string
property_value: skos:example "As for fiat point, fiat line, fiat surface, site" xsd:string

[Term]
id: BFO:0000145
name: relational quality
is_a: BFO:0000019 ! quality
property_value: dce:identifier "057-BFO" xsd:string
property_value: skos:definition "b is a relational quality =Def b is a quality & there exists c and d such that c and d are not identical & b specifically depends on c & b specifically depends on d" xsd:string
property_value: skos:example "A marriage bond; an instance of love; an obligation between one person and another" xsd:string

[Term]
id: BFO:0000146
name: fiat surface
is_a: BFO:0000140 ! continuant fiat boundary
property_value: dce:identifier "033-BFO" xsd:string
property_value: skos:definition "(Elucidation) A fiat surface is a two-dimensional continuant fiat boundary that is self-connected" xsd:string
property_value: skos:example "The surface of the Earth; the plane separating the smoking from the non-smoking zone in a restaurant" xsd:string

[Term]
id: ontologies:GEOCORE_0000001
name: geological object
def: "An object that is 'generated by' some 'geological process' and has at least one part 'constituted by' some 'earth material' that is not an 'earth fluid'." []
is_a: BFO:0000030 ! object
disjoint_from: ontologies:GEOCORE_0000006 ! earth material
relationship: BFO:0000196 ontologies:GEORES_0000022 ! bearer of dimension
relationship: ontologies:GEOCORE_0000015 ontologies:GEOCORE_0000003 ! geological age
property_value: IAO:0000116 "A geological object is a naturally occurring entity because a geological process\ngenerates it, and some earth material constitutes it. Thus, we can differentiate geological objects from artificial objects, such as a well-core, because even though some earth material constitutes artificial objects, they are human-made rather than generated by some geological process. Furthermore, Geological Objects are specializations of BFO Objects, meaning they must necessarily have some unity criteria. The unity is what differentiates geological objects from Earth Materials." xsd:string
property_value: skos:altLabel "objeto geológico" xsd:string

[Term]
id: ontologies:GEOCORE_0000002
name: geological process
def: "It is a physical, or chemical, or biological, naturally occurring process that occurs on the Earth’s surface or subsurface and occupies some 'geological time interval'" []
is_a: BFO:0000015 ! process
relationship: BFO:0000199 ontologies:GEOCORE_0000005 ! occupies temporal region geological time interval
property_value: IAO:0000112 "Examples are the process of deposition, the process of folding, a tectonic process, a sedimentary process." xsd:string
property_value: IAO:0000116 "Geological processes are macro processes that generate, transform, deform, transport, or destroy geological objects and earth materials. These processes are not necessarily atomic and may have other geological processes as parts." xsd:string
property_value: skos:altLabel "processo geológico" xsd:string

[Term]
id: ontologies:GEOCORE_0000003
name: geological age
def: "It is a quality that 'inheres in' a 'geological object' or 'earth material' that corresponds to the 'geological time interval' in which the 'geological process' that it was 'generated by' occupied." []
is_a: BFO:0000019 ! quality
property_value: skos:altLabel "idade geológica" xsd:string

[Term]
id: ontologies:GEOCORE_0000004
name: geological structure
def: "It is a 'generically dependent continuant' that is the pattern of a non-atomic 'geological object''s internal arrangement." []
is_a: BFO:0000031 ! generically dependent continuant
relationship: BFO:0000084 ontologies:GEOCORE_0000001 ! generically depends on geological object
property_value: IAO:0000116 "Geological structures are general material patterns repeated in many geological\nobjects. The pattern comprises the material configuration and the mutual relationships of the object’s different parts. Structures result from one or a series of geological processes that generated or transformed the geological object they generically depend on. Thus, there is some historical dependence relation between the structure and this geological process, but what concretizes the structure is some complex quality inhering in the object, not the process." xsd:string
property_value: skos:altLabel "estrutura geológica" xsd:string

[Term]
id: ontologies:GEOCORE_0000005
name: geological time interval
def: "It is a BFO temporal interval that corresponds to a time interval within the Geological Time Scale." []
is_a: BFO:0000038 ! one-dimensional temporal region
property_value: skos:altLabel "intervalo de tempo geológico" xsd:string

[Term]
id: ontologies:GEOCORE_0000006
name: earth material
def: "It is a natural amount of matter 'generated by' some 'geological process'." []
is_a: BFO:0000040 ! material entity
relationship: ontologies:GEOCORE_0000015 ontologies:GEOCORE_0000003 ! geological age
property_value: IAO:0000112 "Examples are an amount of sandstone, an amount of petroleum, an amount of\nnatural gas." xsd:string
property_value: IAO:0000116 "Earth Materials are natural amounts of matter. Thus, they come into existence by nature, without any artificial aid. Since they are amounts, they don’t hold unity criteria, but they are ontologically rigid and provide an identity criteria. Earth Materials and BFO Objects are disjoint. They are either solid, fluid, or unconsolidated. We usually observe earth materials when constituting other objects, such as an amount of rock constituting a geological unity or an amount of sand constituting a dune." xsd:string
property_value: skos:altLabel "material geologico" xsd:string

[Term]
id: ontologies:GEOCORE_0000007
name: amount of mineral
def: "An amount of rock is an 'earth material' that is a naturally occuring, inorganic, solid, homogeneous chemical compound with a crystalline structure." []
is_a: ontologies:GEOCORE_0000006 ! earth material
disjoint_from: ontologies:GEOCORE_0000008 ! amount of rock
disjoint_from: ontologies:GEOCORE_0000008 ! amount of rock
property_value: IAO:0000112 "The amount of quarts that constitutes some grain, the amount of feldspar that is part of an amount of rock." xsd:string
property_value: IAO:0000116 "Amounts of mineral lack a unity criteria as every other 'earth material'. We usually observe them when they are constitution objects such as crystals or grains." xsd:string
property_value: skos:altLabel "quantidade de mineral" xsd:string

[Term]
id: ontologies:GEOCORE_0000008
name: amount of rock
def: "An amount of rock is a solid consolidated 'earth material' that is 'constituted by' an aggregate of particles made of mineral matter or material of biological origin." []
is_a: ontologies:GEOCORE_0000006 ! earth material
disjoint_from: ontologies:GEOCORE_0000009 ! earth fluid
relationship: BFO:0000196 ontologies:GEORES_0000024 ! bearer of lithology
property_value: IAO:0000112 "The amount of sandstone that constitutes a lithostratigraphic unit." xsd:string
property_value: IAO:0000116 "Geologists define rocks at a scale of observation where they consider them homogeneous, even though an aggregate of solid particles constitutes it. These particles are usually geological objects, such as grains or crystals, or the rest of dead animals or plants. \n\nAmounts of rock, like other earth materials, are independent rigid entities that do not hold any unity criteria. We can observe them in nature when they are constituting objects such as geological unities." xsd:string
property_value: skos:altLabel "quantidade de rocha" xsd:string

[Term]
id: ontologies:GEOCORE_0000009
name: earth fluid
def: "Earth fluid is an 'earth material' that is fluild." []
is_a: ontologies:GEOCORE_0000006 ! earth material
property_value: IAO:0000116 "Earth fluids can be water, oil, gas or a mixture of those fluids." xsd:string
property_value: skos:altLabel "fluido da terra" xsd:string

[Term]
id: ontologies:GEOCORE_0000010
name: unconsolidated earth material
def: "Unconsolidated earth material is an 'earth material' that is consituted by an aggregate of solid particles but is not consolidated into a 'rock' it self." []
is_a: ontologies:GEOCORE_0000006 ! earth material
property_value: skos:altLabel "material geológico inconsolidado" xsd:string

[Term]
id: ontologies:GEOCORE_0000011
name: geological boundary
def: "It is a fiat surface that is 'located in' the external surface of a 'geological object'." []
is_a: BFO:0000146 ! fiat surface
property_value: IAO:0000116 "The 'geological boundary' of a 'geological object' coincides with the complete physical discontinuity that delimits it." xsd:string
property_value: skos:altLabel "limite geológico" xsd:string

[Term]
id: ontologies:GEOCORE_0000012
name: geological contact
def: "It is a 'relational quality' that 'inheres in' two distinct 'geological object' that are 'externally connected with'" []
is_a: BFO:0000145 ! relational quality
relationship: BFO:0000197 ontologies:GEOCORE_0000001 {cardinality="2"} ! inheres in geological object
property_value: IAO:0000116 "A geological contact exists when two distinct geological objects are externally\nconnected with, i.e., their external boundaries are physically adjacent. Objects that are in contact do not have any kind of proper parthood relationship between them." xsd:string
property_value: skos:altLabel "contato geológico" xsd:string

[Term]
id: ontologies:GEORES_0000001
name: body of rock
is_a: ontologies:GEOCORE_0000001 ! geological object
intersection_of: ontologies:GEOCORE_0000001 ! geological object
intersection_of: ontologies:GEOCORE_0000017 ontologies:GEOCORE_0000008 ! amount of rock
relationship: BFO:0000101 ontologies:GEOCORE_0000004 ! is carrier of geological structure
relationship: BFO:0000129 ontologies:GEORES_0000020 ! member part of depositional system
relationship: BFO:0000129 ontologies:GEORES_0000021 ! member part of sedimentary environment
relationship: ontologies:GEOCORE_0000017 ontologies:GEOCORE_0000008 ! amount of rock
property_value: skos:altLabel "corpo de rocha" xsd:string
property_value: skos:definition "'body of rock' is a 'geological object' that is 'constituted by' some 'amount of rock'" xsd:string

[Term]
id: ontologies:GEORES_0000002
name: stratigraphic unit
comment: Os diferentes elementos arquiteturais ocorrem dentro de uma unidade com uma idade definida que é a unidade estratigráfica.\n\nAinda não sabemos se poderia ser uma unidade litoestratigráfica.
is_a: ontologies:GEORES_0000001 ! body of rock
property_value: skos:altLabel "unidade estratigráfica" xsd:string

[Term]
id: ontologies:GEORES_0000003
name: lithostratigraphic unit
is_a: ontologies:GEORES_0000001 ! body of rock
property_value: skos:altLabel "unidade litoestratigráfica" xsd:string

[Term]
id: ontologies:GEORES_0000004
name: formation
is_a: ontologies:GEORES_0000003 ! lithostratigraphic unit
relationship: BFO:0000129 ontologies:GEORES_0000019 ! member part of group
property_value: skos:altLabel "formação" xsd:string

[Term]
id: ontologies:GEORES_0000005
name: member
is_a: ontologies:GEORES_0000003 ! lithostratigraphic unit
relationship: BFO:0000176 ontologies:GEORES_0000004 ! continuant part of formation
property_value: skos:altLabel "membro" xsd:string

[Term]
id: ontologies:GEORES_0000006
name: architectural element
comment: A restrição de partes de escala menores ainda não foi implementada.
comment: Luan: Elementos arquiteturais são os objetos básicos que os geólogos vão reconhecer e descrever. Eles podem ocorrer em diversas escalas.\nUm elemento pode ter outro elemento como parte, desde que de uma escala menor.
is_a: ontologies:GEORES_0000001 ! body of rock
relationship: BFO:0000196 ontologies:GEORES_0000023 ! bearer of geometry
property_value: skos:altLabel "elemento arquitetural" xsd:string

[Term]
id: ontologies:GEORES_0000007
name: build up unit
is_a: ontologies:GEORES_0000006 ! architectural element
disjoint_from: ontologies:GEORES_0000008 ! channel unit
disjoint_from: ontologies:GEORES_0000008 ! channel unit
property_value: skos:altLabel "edifício" xsd:string

[Term]
id: ontologies:GEORES_0000008
name: channel unit
def: "An elongated Depositional Unit having some Channel Surface as its boundary and constituted by some Sediment or Sedimentary Rock that fills it (McHargue et al., 2011)." []
comment: In stratigraphic terms, a channel unit is constituted by the sediments or sedimentary rocks that fill a channel. It is important to notice that, in more general terms, a channel is a passageway for fluids or sediments, i.e., an immaterial entity. If one elaborates about the erosion and deposition processes that generate these units (McHargue et al., 2011), it is essential to have this disambiguation.
comment: In this work, we decided not to model the named hierarchical scales as entities (e.g., Channel Element, Channel Complex, Channel Complex Set - McHargue et al., 2011) because there exists a wide variety of hierarchical schemes in the literature, and they are not necessarily interoperable (Cullis et al., 2018). Instead, we focus on the fact that units can be fractally nested: a unit can be a Proper Spatial Part Of another unit, which can be a Proper Spatial Part Of another unit, and so forth. We consider that this approach solves the problem of implementing a solution for the repeatability of the geological objects in multiple scales. As so, a Channel Unit can be decomposed in other Channel Units many times as necessary, keeping the representation structure. In the future, we can study the integration of hierarchical schemes and try to infer scales from the spatial relations.
is_a: ontologies:GEORES_0000006 ! architectural element
disjoint_from: ontologies:GEORES_0000013 ! levee unit
property_value: ontologies:GEORES_0000050 "R+ I+ O- U+ ED-" xsd:string
property_value: skos:altLabel "canal" xsd:string

[Term]
id: ontologies:GEORES_0000009
name: dome unit
is_a: ontologies:GEORES_0000006 ! architectural element
property_value: skos:altLabel "domo" xsd:string

[Term]
id: ontologies:GEORES_0000010
name: dune unit
is_a: ontologies:GEORES_0000006 ! architectural element
property_value: skos:altLabel "campo de dunas" xsd:string

[Term]
id: ontologies:GEORES_0000011
name: intrusive dike
is_a: ontologies:GEORES_0000006 ! architectural element
property_value: skos:altLabel "dique intrusivo" xsd:string

[Term]
id: ontologies:GEORES_0000012
name: intrusive sill unit
is_a: ontologies:GEORES_0000006 ! architectural element
property_value: skos:altLabel "soleira intrusiva" xsd:string

[Term]
id: ontologies:GEORES_0000013
name: levee unit
def: "A Depositional Unit having Wedge Geometry and forming a bank or ridge geomorphology associated with some Channel Unit." []
comment: This term is not consensual as some authors refer to these units as the wedge-shape embankments around channels, which is the definition that we adopt here, while other authors refer to them as not necessarily being these embankments and possibly having wing shapes, among other definitions.
comment: This term refers to the geomorphological association of some wegde-shaped unit with some channel unit, even if the channel does not exist at the moment of the observation by the geologist and the levee is probabilistically identified by tendencies (e.g., typical facies). In other words, the term "levee" ontologicallly denotes this relation even though it cannot be deterministically observed.
is_a: ontologies:GEORES_0000006 ! architectural element
property_value: ontologies:GEORES_0000050 "R~ I+ O- U+ ED-" xsd:string
property_value: skos:altLabel "dique" xsd:string

[Term]
id: ontologies:GEORES_0000014
name: lobe unit
def: "A Depositional Unit having some Lobe Geometry." []
comment: For Lobe Unit hierarchical scales, we adopted the same approach as in Channel Unit.
comment: These depositional units are usually found at deep-water depositional system terminal regions, or at channel laterals as Overbank Units.
is_a: ontologies:GEORES_0000006 ! architectural element
property_value: ontologies:GEORES_0000050 "R+ I+ O- U+ ED-" xsd:string
property_value: skos:altLabel "lobo" xsd:string

[Term]
id: ontologies:GEORES_0000015
name: mound unit
def: "A Depositional Unit having Mound Geometry with an irregular top surface and internal chaotic facies." []
is_a: ontologies:GEORES_0000006 ! architectural element
property_value: ontologies:GEORES_0000050 "R+ I+ O- U+ ED-" xsd:string
property_value: skos:altLabel "monte" xsd:string

[Term]
id: ontologies:GEORES_0000016
name: olistrostomes unit
is_a: ontologies:GEORES_0000006 ! architectural element
property_value: IAO:0000118 "megaclast" xsd:string
property_value: IAO:0000118 "megaclasto" xsd:string
property_value: skos:altLabel "olistrostomas" xsd:string

[Term]
id: ontologies:GEORES_0000017
name: sheet unit
is_a: ontologies:GEORES_0000006 ! architectural element
property_value: skos:altLabel "lençol" xsd:string

[Term]
id: ontologies:GEORES_0000018
name: fossil
is_a: ontologies:GEOCORE_0000001 ! geological object
property_value: skos:altLabel "fóssil" xsd:string

[Term]
id: ontologies:GEORES_0000019
name: group
is_a: BFO:0000027 ! object aggregate
relationship: BFO:0000115 ontologies:GEORES_0000004 {all_only="true"} ! has member part formation
property_value: skos:altLabel "grupo" xsd:string

[Term]
id: ontologies:GEORES_0000020
name: depositional system
def: "An Object Aggregate whose members are mereotopologically-linked Depositional Units." []
is_a: BFO:0000027 ! object aggregate
property_value: ontologies:GEORES_0000050 "R+ I+ O+ U+ ED-" xsd:string
property_value: skos:altLabel "sistema deposicional" xsd:string

[Term]
id: ontologies:GEORES_0000021
name: sedimentary environment
def: "The sedimentary environment is the specific depositional setting of a particular sedimentary rock and is unique in terms of physical, chemical, and biological characteristics." []
is_a: BFO:0000027 ! object aggregate
property_value: IAO:0000119 "Britannica\nhttps://www.britannica.com/science/sedimentary-rock/Sedimentary-environments" xsd:string
property_value: skos:altLabel "ambiente de sedimentação" xsd:string

[Term]
id: ontologies:GEORES_0000022
name: dimension
def: "A Quality that inheres in an Independent Continuant by virtue of one of its one-dimensional extents. It is a category that includes at least the three dimensions defined in this ontology: Width, Length, and Thickness. All dimensions are expressed by a real number indicating its value and a literal string indicating its measurement unit." []
is_a: BFO:0000019 ! quality

[Term]
id: ontologies:GEORES_0000023
name: geometry
def: "A Quality that inheres in a Depositional Unit by virtue of its external three-dimensional shape. It does not reflect the exact mathematical specifications of a geometric shape but abstracts and simplifies these specifications (Rovetto, 2011)." []
is_a: BFO:0000019 ! quality
relationship: ontologies:GEORES_0000046 ontologies:GEORES_0000042 {minCardinality="1"} ! geometry type
property_value: skos:altLabel "geometria" xsd:string

[Term]
id: ontologies:GEORES_0000024
name: lithology
is_a: BFO:0000019 ! quality
property_value: skos:altLabel "litologia" xsd:string

[Term]
id: ontologies:GEORES_0000025
name: statigraphic contact
is_a: ontologies:GEOCORE_0000012 ! geological contact
property_value: skos:altLabel "contato estratigráfico" xsd:string

[Term]
id: ontologies:GEORES_0000026
name: bed contact
is_a: ontologies:GEOCORE_0000012 ! geological contact
relationship: ontologies:GEORES_0000044 ontologies:GEORES_0000041 {cardinality="1"} ! contact position
relationship: ontologies:GEORES_0000045 ontologies:GEORES_0000043 {cardinality="1"} ! contact type
property_value: skos:altLabel "contato de camada" xsd:string

[Term]
id: ontologies:GEORES_0000027
name: sinuosity
def: "A Quality that inheres in a Channel Unit by virtue of how wavy it is across its length. It is expressed by a real number given by its curved length divided by its length in a straight line." []
is_a: BFO:0000019 ! quality
relationship: BFO:0000197 ontologies:GEORES_0000008 {cardinality="1"} ! inheres in channel unit

[Term]
id: ontologies:GEORES_0000028
name: facies
def: "A pattern of properties of Geological Objects." []
comment: This entity is defined in the literature as a combination of features that differentiates a geological object from its adjacent geological objects (Walker and James, 1992). However, a Facies does not describe a single Geological Object’s features: it might repeat in several objects as a pattern. This particular aspect matches the definition of Generically Dependent Continuant in BFO. Another important aspect is that the features that compose facies vary depending on the research context, e.g., Sedimentary Facies, Petrofacies (De Ros and Goldberg, 2007), Lithofacies, Ichnofacies, and Biofacies (Nichols, 2009).
is_a: BFO:0000031 ! generically dependent continuant
relationship: BFO:0000084 ontologies:GEORES_0000001 ! generically depends on body of rock
property_value: skos:altLabel "fácies" xsd:string

[Term]
id: ontologies:GEORES_0000029
name: sedimentary facies
def: "A Facies consisting of the sum of the sedimentological characteristics of Depositional Units (Middleton, 1973, Nichols, 2009, Carbonera et al., 2015)." []
comment: As an example, if we would model Cross-bedded Sandstone (Nichols, 2009), it would be an entity subsumed by Sedimentary Facies having the following relations: (1) Generically Depends On some (Constituted By some Sandstone (a)); and (2) Has Part some Cross-bedding Structure (b). (a): Sandstone would be an entity subsumed by Sedimentary Rock. (b): Cross-bedding Structure would be an entity subsumed by Sedimentary Structure.
is_a: ontologies:GEORES_0000028 ! facies
property_value: skos:altLabel "fácies sedimentar" xsd:string

[Term]
id: ontologies:GEORES_0000030
name: facies association
def: "A Generically Dependent Continuant that consists of an aggregate of Facies." []
comment: It usually describes the Facies that are typically found in specific regions or sub-environments. For example, the Channel Axis Association (McHargue et al., 2011) describes Sedimentary Facies typically found at the center part of channels (in a cross-section point of view).
is_a: BFO:0000031 ! generically dependent continuant
relationship: BFO:0000178 ontologies:GEORES_0000028 {minCardinality="2"} ! has continuant part facies
property_value: skos:altLabel "associação de facies" xsd:string

[Term]
id: ontologies:GEORES_0000031
name: sediment
def: "An Unconsolidated Earth Material constituted by some collection of sedimentary grains or particles (Garcia et al., 2019)." []
is_a: ontologies:GEOCORE_0000010 ! unconsolidated earth material
property_value: ontologies:GEORES_0000050 "R+ I+ O- U- ED-" xsd:string

[Term]
id: ontologies:GEORES_0000032
name: sedimentary rock
def: "'sedimentary rock' is an 'amount of rock' constituted by some collection of sedimentary grains or particles (Garcia et al., 2019)." []
is_a: ontologies:GEOCORE_0000008 ! amount of rock
disjoint_from: ontologies:GEORES_0000033 ! igneous rock
property_value: ontologies:GEORES_0000050 "R+ I+ O- U- ED-" xsd:string
property_value: skos:altLabel "rocha sedimentar" xsd:string

[Term]
id: ontologies:GEORES_0000033
name: igneous rock
is_a: ontologies:GEOCORE_0000008 ! amount of rock
property_value: isDefinedBy "https://www.britannica.com/science/igneous-rock" xsd:string
property_value: skos:altLabel "rocha ígnea" xsd:string
property_value: skos:definition "'igneous rock' is an 'amount of rock' generated by the cooling and solidification of molten 'earth material'." xsd:string

[Term]
id: ontologies:GEORES_0000034
name: metamorphic rock
is_a: ontologies:GEOCORE_0000008 ! amount of rock
property_value: isDefinedBy "Adapted from Brittanica.\nhttps://www.britannica.com/science/metamorphic-rock" xsd:string
property_value: skos:altLabel "rocha metamórfica" xsd:string
property_value: skos:definition "'metamorphic rock' is an 'amount of rock' generated by the alteration of preexisting rocks in response to changing environmental conditions, such as variations in temperature, pressure, and mechanical stress, and the addition or subtraction of chemical components." xsd:string

[Term]
id: ontologies:GEORES_0000035
name: complex architectural element
is_a: ontologies:GEORES_0000001 ! body of rock
disjoint_from: ontologies:GEORES_0000036 ! composite architectural element

[Term]
id: ontologies:GEORES_0000036
name: composite architectural element
is_a: ontologies:GEORES_0000001 ! body of rock

[Term]
id: ontologies:GEORES_0000037
name: individual architectural element

[Term]
id: ontologies:GEORES_0000038
name: channel surface
def: "A Geological Boundary that forms the basis of a Channel Unit, having a concave-up shape unless truncated by overlying depositional units." []
is_a: ontologies:GEOCORE_0000011 ! geological boundary
property_value: ontologies:GEORES_0000050 "R+ I+ O- U+ ED-" xsd:string

[Term]
id: ontologies:GEORES_0000039
name: basin
is_a: BFO:0000029 ! site
property_value: skos:altLabel "bacia" xsd:string

[Term]
id: ontologies:GEORES_0000040
name: geological site
comment: Epistemologicamente não é possível determinar os limites deste site e, portanto, cada geólogo pode posicionar sua área de interesse em uma localização e limites distintos, o que torna muito difícil tratar computacionalmente a identidade do sítio geológico. Esse problema acontece com outras entidades do tipo site: Região da Serra Gaúcha, Litoral Norte, etc, cuja delimitação é problemática, mas existe uma identidade consensual.
is_a: BFO:0000029 ! site
property_value: skos:altLabel "sítio geológico" xsd:string

[Term]
id: ontologies:GEORES_0000041
name: contact position
is_a: BFO:0000001 ! entity
property_value: skos:altLabel "posição do contato" xsd:string

[Term]
id: ontologies:GEORES_0000042
name: geometry type
comment: Luan: Talvez tipo de Geometria seja uma classe de segunda ordem, mas em primeiro momento não utilizaremos punning para representar isto. A classe geometry tem uma relação de 'has geometry type' com um 'geometry type' e as instâncias dessa classe é que definem o tipo de geometria de fato. Caso seja necessário criar alguma subclasse de um 'body of rock' que tenha um 'geometry type' específico é possível utilizar a primitiva do owl value para isto.\n\nNão sabemos ainda como classificar esta classe. Do que ela seria subclasse?
is_a: BFO:0000001 ! entity
property_value: skos:altLabel "tipo de geometria" xsd:string

[Term]
id: ontologies:GEORES_0000043
name: contact type
is_a: BFO:0000001 ! entity
property_value: skos:altLabel "tipo de contato" xsd:string

[Term]
id: ontologies:GEORES_0000075
name: extravasamento
is_a: ontologies:GEORES_0000006 ! architectural element
property_value: skos:altLabel "extravasamento" xsd:string

[Term]
id: ontologies:GEORES_0000076
name: extravasamento interno conectado
is_a: ontologies:GEORES_0000089 ! extravasamento conectado
disjoint_from: ontologies:GEORES_0000077 ! extravasamento externo conectado
property_value: skos:altLabel "extravasamento interno conectado" xsd:string

[Term]
id: ontologies:GEORES_0000077
name: extravasamento externo conectado
is_a: ontologies:GEORES_0000089 ! extravasamento conectado
property_value: skos:altLabel "extravasamento externo conectado" xsd:string

[Term]
id: ontologies:GEORES_0000078
name: espraiamento
is_a: ontologies:GEORES_0000006 ! architectural element
property_value: skos:altLabel "espraiamento" xsd:string

[Term]
id: ontologies:GEORES_0000079
name: espraiamento lateral
is_a: ontologies:GEORES_0000078 ! espraiamento
disjoint_from: ontologies:GEORES_0000080 ! espraiamento terminal
property_value: skos:altLabel "espraiamento lateral" xsd:string

[Term]
id: ontologies:GEORES_0000080
name: espraiamento terminal
is_a: ontologies:GEORES_0000078 ! espraiamento
property_value: skos:altLabel "espraiamento terminal" xsd:string

[Term]
id: ontologies:GEORES_0000081
name: espraiamento capturado
is_a: ontologies:GEORES_0000078 ! espraiamento

[Term]
id: ontologies:GEORES_0000082
name: mass transport deposit
name: transporte de massa
is_a: ontologies:GEORES_0000006 ! architectural element

[Term]
id: ontologies:GEORES_0000083
name: acobertamento
is_a: ontologies:GEORES_0000006 ! architectural element

[Term]
id: ontologies:GEORES_0000084
name: canal degradacional
is_a: ontologies:GEORES_0000008 ! channel unit
disjoint_from: ontologies:GEORES_0000085 ! canal agradacional
disjoint_from: ontologies:GEORES_0000085 ! canal agradacional
property_value: skos:altLabel "canal degradacional" xsd:string

[Term]
id: ontologies:GEORES_0000085
name: canal agradacional
is_a: ontologies:GEORES_0000008 ! channel unit
property_value: skos:altLabel "canal agradacional" xsd:string

[Term]
id: ontologies:GEORES_0000086
name: canal neutro
is_a: ontologies:GEORES_0000008 ! channel unit
property_value: skos:altLabel "canal neutro" xsd:string

[Term]
id: ontologies:GEORES_0000087
name: cunha de contorno
is_a: ontologies:GEORES_0000006 ! architectural element
property_value: skos:altLabel "cunha de contorno" xsd:string

[Term]
id: ontologies:GEORES_0000088
name: zona de transição canal-espraiamento
is_a: ontologies:GEORES_0000006 ! architectural element
property_value: skos:altLabel "zona de transição canal-espraiamento" xsd:string

[Term]
id: ontologies:GEORES_0000089
name: extravasamento conectado
is_a: ontologies:GEORES_0000075 ! extravasamento
disjoint_from: ontologies:GEORES_0000090 ! extravasamento descontectado
property_value: skos:altLabel "extravasamento conectado" xsd:string

[Term]
id: ontologies:GEORES_0000090
name: extravasamento descontectado
is_a: ontologies:GEORES_0000075 ! extravasamento
property_value: skos:altLabel "extravasamento descontectado" xsd:string

[Term]
id: ontologies:GEORES_0000091
name: extravasamento interno descontectado
is_a: ontologies:GEORES_0000090 ! extravasamento descontectado
disjoint_from: ontologies:GEORES_0000092 ! extravasamento externo desconectado
property_value: skos:altLabel "extravasamento interno descontectado" xsd:string

[Term]
id: ontologies:GEORES_0000092
name: extravasamento externo desconectado
is_a: ontologies:GEORES_0000090 ! extravasamento descontectado
property_value: skos:altLabel "extravasamento externo desconectado" xsd:string

[Term]
id: ontologies:GEORES_0000093
name: acobertamento local
is_a: ontologies:GEORES_0000083 ! acobertamento
disjoint_from: ontologies:GEORES_0000094 ! acobertamento regional

[Term]
id: ontologies:GEORES_0000094
name: acobertamento regional
is_a: ontologies:GEORES_0000083 ! acobertamento
property_value: skos:altLabel "acobertamento regional" xsd:string

[Typedef]
id: BFO:0000084
name: generically depends on
property_value: dce:identifier "252-BFO" xsd:string
property_value: skos:altLabel "g-depends on" xsd:string
property_value: skos:definition "b generically depends on c =Def b is a generically dependent continuant & c is an independent continuant that is not a spatial region & at some time t there inheres in c a specifically dependent continuant which concretizes b at t" xsd:string
property_value: skos:scopeNote "Users that require more sophisticated representations of time are encouraged to import a temporal extension of BFO-Core provided by the BFO development team. See documentation for guidance: <Link>" xsd:string
domain: BFO:0000031 ! generically dependent continuant
inverse_of: BFO:0000101 ! is carrier of

[Typedef]
id: BFO:0000101
name: is carrier of
property_value: dce:identifier "254-BFO" xsd:string
property_value: skos:definition "b is carrier of c =Def there is some time t such that c generically depends on b at t" xsd:string
property_value: skos:scopeNote "Users that require more sophisticated representations of time are encouraged to import a temporal extension of BFO-Core provided by the BFO development team. See documentation for guidance: <Link>" xsd:string
range: BFO:0000031 ! generically dependent continuant

[Typedef]
id: BFO:0000115
name: has member part
property_value: dce:identifier "230-BFO" xsd:string
property_value: skos:definition "b has member part c =Def c member part of b" xsd:string
property_value: skos:scopeNote "Users that require more sophisticated representations of time are encouraged to import a temporal extension of BFO-Core provided by the BFO development team. See documentation for guidance: <Link>" xsd:string
domain: BFO:0000040 ! material entity
range: BFO:0000040 ! material entity
is_a: BFO:0000178 ! has continuant part
inverse_of: BFO:0000129 ! member part of

[Typedef]
id: BFO:0000129
name: member part of
property_value: dce:identifier "228-BFO" xsd:string
property_value: skos:definition "b member part of c =Def b is an object & c is a material entity & there is some time t such that b continuant part of c at t & there is a mutually exhaustive and pairwise disjoint partition of c into objects x1, ..., xn (for some n ≠ 1) with b = xi (for some 1 <= i <= n)" xsd:string
property_value: skos:scopeNote "Users that require more sophisticated representations of time are encouraged to import a temporal extension of BFO-Core provided by the BFO development team. See documentation for guidance: <Link>" xsd:string
domain: BFO:0000040 ! material entity
range: BFO:0000040 ! material entity
is_a: BFO:0000176 ! continuant part of

[Typedef]
id: BFO:0000176
name: continuant part of
property_value: dce:identifier "221-BFO" xsd:string
property_value: skos:definition "b continuant part of c =Def b and c are continuants & there is some time t such that b and c exist at t & b continuant part of c at t" xsd:string
property_value: skos:example "Milk teeth continuant part of human; surgically removed tumour continuant part of organism" xsd:string
property_value: skos:scopeNote "Users that require more sophisticated representations of time are encouraged to import a temporal extension of BFO-Core provided by the BFO development team. See documentation for guidance: <Link>" xsd:string
domain: BFO:0000002 ! continuant
range: BFO:0000002 ! continuant
inverse_of: BFO:0000178 ! has continuant part

[Typedef]
id: BFO:0000178
name: has continuant part
property_value: dce:identifier "271-BFO" xsd:string
property_value: skos:definition "b has continuant part c =Def c continuant part of b" xsd:string
property_value: skos:scopeNote "Users that require more sophisticated representations of time are encouraged to import a temporal extension of BFO-Core provided by the BFO development team. See documentation for guidance: <Link>" xsd:string
domain: BFO:0000002 ! continuant
range: BFO:0000002 ! continuant

[Typedef]
id: BFO:0000194
name: specifically depended on by
property_value: dce:identifier "260-BFO" xsd:string
property_value: skos:altLabel "s-depended on by" xsd:string
property_value: skos:definition "b specifically depended on by c =Def c specifically depends on b" xsd:string
property_value: skos:example "Coloured object specifically depended on by colour" xsd:string
range: BFO:0000020 ! specifically dependent continuant
inverse_of: BFO:0000195 ! specifically depends on

[Typedef]
id: BFO:0000195
name: specifically depends on
property_value: dce:identifier "012-BFO" xsd:string
property_value: skos:altLabel "s-depends on" xsd:string
property_value: skos:definition "(Elucidation) specifically depends on is a relation between a specifically dependent continuant b and specifically dependent continuant or independent continuant that is not a spatial region c such that b and c share no parts in common & b is of a nature such that at all times t it cannot exist unless c exists & b is not a boundary of c" xsd:string
property_value: skos:example "A shape specifically depends on the shaped object; hue, saturation and brightness of a colour sample specifically depends on each other" xsd:string
property_value: skos:scopeNote "The analogue of specifically depends on for occurrents is has participant." xsd:string
domain: BFO:0000020 ! specifically dependent continuant

[Typedef]
id: BFO:0000196
name: bearer of
property_value: dce:identifier "053-BFO" xsd:string
property_value: skos:definition "b bearer of c =Def c inheres in b" xsd:string
property_value: skos:example "A patch of ink is the bearer of a colour quality; an organism is the bearer of a temperature quality" xsd:string
range: BFO:0000020 ! specifically dependent continuant
is_a: BFO:0000194 ! specifically depended on by
inverse_of: BFO:0000197 ! inheres in

[Typedef]
id: BFO:0000197
name: inheres in
property_value: dce:identifier "051-BFO" xsd:string
property_value: skos:definition "b inheres in c =Def b is a specifically dependent continuant & c is an independent continuant that is not a spatial region & b specifically depends on c" xsd:string
property_value: skos:example "A shape inheres in a shaped object; a mass inheres in a material entity" xsd:string
domain: BFO:0000020 ! specifically dependent continuant
is_a: BFO:0000195 ! specifically depends on

[Typedef]
id: BFO:0000199
name: occupies temporal region
property_value: dce:identifier "132-BFO" xsd:string
property_value: skos:definition "p occupies temporal region t =Def p is a process or process boundary & the spatiotemporal region occupied by p temporally projects onto t" xsd:string
property_value: skos:example "The Second World War occupies the temporal region September 1, 1939 - September 2, 1945" xsd:string
range: BFO:0000008 ! temporal region
is_functional: true

[Typedef]
id: ontologies:GEOCORE_0000015
name: has age
def: "The relation between a Geological Object and its Geological Age." []
is_a: BFO:0000196 ! bearer of
inverse_of: ontologies:GEOCORE_0000016 ! age of

[Typedef]
id: ontologies:GEOCORE_0000016
name: age of
def: "The relation between a Geological Age and a Geological Object. Inverse of has age relation." []
is_a: BFO:0000197 ! inheres in

[Typedef]
id: ontologies:GEOCORE_0000017
name: constituted by
def: "The relation between some material entity and the material that it is made of." []
property_value: IAO:0000116 "This is a material constitution relation intended to represent the relationship between material objects, such as geological objects and earth materials, or aggregates of them." xsd:string
property_value: IAO:0000119 "Evnine, S. J. (2011). Constitution and composition: Three approaches to their relation. ProtoSociology, 27, 212-235." xsd:string
is_asymmetric: true

[Typedef]
id: ontologies:GEORES_0000044
name: has contact position
domain: ontologies:GEORES_0000026 ! bed contact
range: ontologies:GEORES_0000041 ! contact position

[Typedef]
id: ontologies:GEORES_0000045
name: has contact type
domain: ontologies:GEORES_0000026 ! bed contact
range: ontologies:GEORES_0000043 ! contact type

[Typedef]
id: ontologies:GEORES_0000046
name: has geometry type
comment: Luan: Geometry Type talvez seja uma classe de segunda ordem cuja as instâncias são os diferentes tipos de Geometria. Por exemplo, é errado dizer que Geometria Lenticular é subtipo da Quality Geometria. Lenticular é na realidade um subtipo de Tipo de Geometria e não de Geometria.
domain: ontologies:GEORES_0000023 ! geometry
range: ontologies:GEORES_0000042 ! geometry type

[Typedef]
id: ontologies:GEORES_0000047
name: has base geometry
is_a: ontologies:GEORES_0000046 ! has geometry type

[Typedef]
id: ontologies:GEORES_0000048
name: has top geometry
is_a: ontologies:GEORES_0000046 ! has geometry type

